src/lib/poly/gemm/Kuiper.Poly.GEMM.TensorCore2D.fst
@@ -544,8 +544,11 @@ fn kf
   // Assumming functional correctness
   with tC'.
     assert warp_tile_pts_to gC bm bn tm tn wm wn bid (tid / warp_size) tC';
-  assume pure (tC' %~ MS.matmul (ematrix_subtile rA (wm*tm) shared (warp_tile_i #rows #cols bm bn bk tm tn tk wm wn nthr bid tid) 0)
-                                (ematrix_subtile rB shared  (wn*tn) 0 (warp_tile_j #rows #cols bm bn bk tm tn tk wm wn nthr bid tid)));
+  assume pure (tC' %~ MS.matmul (ematrix_subtile rA (wm*tm) shared (warp_tile_i #rows #cols bm bn bk tm tn tk wm wn nthr bid (tid / warp_size)) 0)
+                                (ematrix_subtile rB shared  (wn*tn) 0 (warp_tile_j #rows #cols bm bn bk tm tn tk wm wn nthr bid (tid / warp_size))));
+  fold warp_tile_approximates gC bm bn tm tn wm wn bid (tid / warp_size)
+        (MS.matmul (ematrix_subtile rA (wm*tm) shared (warp_tile_i #rows #cols bm bn bk tm tn tk wm wn nthr bid (tid / warp_size)) 0)
+                  (ematrix_subtile rB shared  (wn*tn) 0 (warp_tile_j #rows #cols bm bn bk tm tn tk wm wn nthr bid (tid / warp_size))));
 
   ()
 }
